

MATH 140 Quiz 5 (Home)

2.5

17) $y(x) = (2x-3)^4 (x^2+x+1)^5$

$$\begin{aligned} y'(x) &= 4(2x-3)^3(2)(x^2+x+1)^5 + (2x-3)^4 \cdot 5(x^2+x+1)^4(2x+1) \\ &= 8(2x-3)^3(x^2+x+1)^5 + (10x+5)(2x-3)^4(x^2+x+1)^4 \end{aligned}$$

25) $h(\theta) = \tan(\theta^2 \sin \theta)$

$$\begin{aligned} h'(\theta) &= \sec^2(\theta^2 \sin \theta) \cdot \frac{d}{d\theta}(\theta^2 \sin \theta) \\ &= \sec^2(\theta^2 \sin \theta) \cdot [2\theta \sin \theta + \theta^2 \cos \theta] \end{aligned}$$

27) $y = \frac{\cos x}{\sqrt{1+\sin x}}$

$$y' = \frac{\sqrt{1+\sin x}(-\sin x) - \cos x \left(\frac{1}{2\sqrt{1+\sin x}} \cdot \cos x \right)}{(\sqrt{1+\sin x})^2}$$

$$= \frac{-\sin x \sqrt{1+\sin x} - \cos^2 x \left(\frac{1}{2\sqrt{1+\sin x}} \right)}{1+\sin x}$$

$$= \frac{-2\sin x(1+\sin x) - \cos^2 x}{2(1+\sin x)^{3/2}}$$

$$= \frac{-2\sin x - 2\sin^2 x - \cos^2 x}{2(1+\sin x)^{3/2}} = -\left(\frac{1+2\sin x + \sin^2 x}{2(1+\sin x)^{3/2}} \right)$$

$$37) \quad y = \cot^2(\sin\theta) = [\cot(\sin\theta)]^2$$

$$\begin{aligned} \frac{dy}{d\theta} &= 2\cot(\sin\theta) \cdot \frac{d}{d\theta}[\cot(\sin\theta)] \\ &= 2\cot(\sin\theta) \cdot (-\csc^2(\sin\theta) \cdot \frac{d}{d\theta}(\sin\theta)) \\ &= -2\cot(\sin\theta) \cdot \csc^2(\sin\theta) \cdot \cos\theta \end{aligned}$$

2.6

$$7) \quad x^4 + x^2y^2 + y^3 = 5$$

$$\Rightarrow 4x^3 + [2xy^2 + x^2(2y\frac{dy}{dx})] + 3y^2\frac{dy}{dx} = 0$$

$$2x^2y\frac{dy}{dx} + 3y^2\frac{dy}{dx} = -4x^3 - 2xy^2$$

$$\frac{dy}{dx} = \frac{-4x^3 - 2xy^2}{2x^2y + 3y^2}$$

$$13) \quad \sqrt{x+y} = x^4 + y^4$$

$$\Rightarrow \frac{1}{2\sqrt{x+y}} \cdot (1 + \frac{dy}{dx}) = 4x^3 + 4y^3\frac{dy}{dx}$$

$$1 + \frac{dy}{dx} = 8x^3\sqrt{x+y} + 8y^3\sqrt{x+y} \cdot \frac{dy}{dx}$$

$$\frac{dy}{dx} - 8y^3\sqrt{x+y} \cdot \frac{dy}{dx} = 8x^3\sqrt{x+y} - 1$$

$$\frac{dy}{dx} = \frac{8x^3\sqrt{x+y} - 1}{1 - 8y^3\sqrt{x+y}}$$

$$19) \sin(xy) = \cos(x+y)$$

$$\Rightarrow \cos(xy) \left[y + x \frac{dy}{dx} \right] = -\sin(x+y) \cdot \left[1 + \frac{dy}{dx} \right]$$

$$y \cos(xy) + x \cos(xy) \frac{dy}{dx} = -\sin(x+y) - \sin(x+y) \frac{dy}{dx}$$

$$x \cos(xy) \frac{dy}{dx} + \sin(x+y) \frac{dy}{dx} = -y \cos(xy) - \sin(x+y)$$

$$\frac{dy}{dx} = \frac{-y \cos(xy) - \sin(x+y)}{x \cos(xy) + \sin(x+y)}$$

$$31) 2(x^2+y^2)^2 = 25(x^2-y^2), \quad (3, 1)$$

$$4(x^2+y^2) \left[2x + 2y \frac{dy}{dx} \right] = \cancel{25} 50x - 50y \frac{dy}{dx}$$

$$\xrightarrow{x=3, y=1} 4(9+1) \left[6 + 2 \frac{dy}{dx} \right] = 150 - 50 \frac{dy}{dx}$$

$$240 + 80 \frac{dy}{dx} = 150 - 50 \frac{dy}{dx}$$

$$130 \frac{dy}{dx} = -90$$

$$\Rightarrow \text{slope} = -\frac{9}{13}$$

$$\text{Equation: } \boxed{y-1 = -\frac{9}{13}(x-3)}$$